Common.v
@@ -1,0 +1,6 @@
+Class Env {K V: Type}: Type :=
+  { env_t: Type;
+    getenv: env_t -> K -> option V;
+    putenv: env_t -> K -> V -> env_t }.
+Arguments Env : clear implicits.
+Arguments env_t {_ _}.
