Semantics.v
@@ -1,5 +1,5 @@
 Require Import Coq.Lists.List.
-Require Import SGA.Syntax.
+Require Import SGA.Common SGA.Syntax.
 
 Import ListNotations.
 
@@ -7,16 +7,30 @@ Inductive value :=
 | vtt
 | vbits (bits: list bool).
 
-Definition opt_bind {A B} (o: option A) (f: A -> option B) :=
-  match o with
-  | Some a => f a
-  | None => None
+Inductive result {A} :=
+| Success (a: A)
+| CannotRun
+| Stuck.
+Arguments result : clear implicits.
+
+Definition result_bind {A B} (r: result A) (f: A -> result B) :=
+  match r with
+  | Success a => f a
+  | CannotRun => CannotRun
+  | Stuck => Stuck
   end.
 
-Definition opt_map {A B} (o: option A) (f: A -> B) :=
-  opt_bind o (fun a => Some (f a)).
+Definition result_map {A B} (r: result A) (f: A -> B) :=
+  result_bind r (fun a => Success (f a)).
 
-Axiom magic : forall {A B} (_: B), A.
+Definition opt_result {A} (default: result A) (o: option A) :=
+  match o with
+  | Some a => Success a
+  | None => default
+  end.
+
+(* Definition bool_result (default: result unit) (b: bool) := *)
+(*   if b then Success tt else default. *)
 
 (* Inductive ReadLogEntry := *)
 (* | LogRead (level: Level) (vec: nat) (idx: nat). *)
@@ -30,82 +44,124 @@ Axiom magic : forall {A B} (_: B), A.
 
 (* Scheme Equality for Level. *)
 
-Inductive LogEntry :=
-| LogRead (level: Level) (vec: nat) (idx: nat)
-| LogWrite (level: Level) (vec: nat) (idx: nat) (val: value).
+Inductive LogEntryKind := LogRead | LogWrite.
+Record LogEntry := LE
+  { kind: LogEntryKind;
+    level: Level;
+    reg: nat;
+    val: value (* vtt for reads *) }.
 
 Definition Log := list LogEntry.
-
-Class Env {K V: Type}: Type :=
-  { tenv: Type;
-    getenv: tenv -> K -> option V;
-    putenv: tenv -> K -> V -> tenv }.
-Arguments Env : clear implicits.
-Arguments tenv {_ _}.
 
 Section Interp.
   Context {TVar: Type}.
   Context {TFn: Type}.
 
-  Context (GammaEnv: Env TVar value).
-  Context (SigmaEnv: Env TFn (list value -> option value)).
+  Context {GammaEnv: Env TVar value}.
+  Context {SigmaEnv: Env TFn (list value -> option value)}.
+  Open Scope bool_scope.
 
-  Context (Sigma: SigmaEnv.(tenv)).
-  Context (V: SigmaEnv.(tenv)).
-  Context (sched_log: Log).
+  Definition log_find log reg (f: LogEntryKind -> Level -> value -> bool) :=
+    List.find (fun '(LE kind lvl r v) => (Nat.eqb reg r) && f kind lvl v) log.
+
+  Definition log_existsb log reg (f: LogEntryKind -> Level -> value -> bool) :=
+    List.existsb (fun '(LE kind lvl r v) => (Nat.eqb reg r) && f kind lvl v) log.
+
+  Definition may_read0 sched_log rule_log idx :=
+    if (log_existsb sched_log idx
+                    (fun kind lvl _ => match kind, lvl with
+                                    | LogWrite, P0 => true
+                                    | _, _ => false
+                                    end)) ||
+       (log_existsb (sched_log ++ rule_log) idx
+                    (fun kind lvl _ => match kind, lvl with
+                                    | _, P1 => true
+                                    | _, _ => false
+                                    end))
+    then CannotRun
+    else Success tt.
+
+  Definition may_read1 sched_log rule_log idx :=
+    if (log_existsb sched_log idx
+                    (fun kind lvl _ => match kind, lvl with
+                                    | LogWrite, P1 => true
+                                    | _, _ => false
+                                    end))
+    then CannotRun
+    else match log_find (rule_log ++ sched_log) idx
+                        (fun kind lvl _ => match kind, lvl with
+                                        | LogWrite, P0 => true
+                                        | _, _ => false
+                                        end) with
+         | Some (LE kind lvl reg v) => Success (Some v)
+         | None => Success None
+         end.
+
+  Definition may_write sched_log rule_log lvl idx :=
+    if match lvl with
+       | P0 => (log_existsb (sched_log ++ rule_log) idx
+                           (fun kind lvl _ => match kind, lvl with
+                                           | LogRead, P1 | LogWrite, _ => true
+                                           | _, _ => false
+                                           end))
+       | P1 => (log_existsb (sched_log ++ rule_log) idx
+                           (fun kind lvl _ => match kind, lvl with
+                                           | LogWrite, P1 => true
+                                           | _, _ => false
+                                           end)) end
+    then CannotRun
+    else Success tt.
 
   Fixpoint interp
-           (Gamma: GammaEnv.(tenv))
+           (Sigma: SigmaEnv.(env_t))
+           (Gamma: GammaEnv.(env_t))
+           (V: list value)
+           (sched_log: Log)
            (rule_log: Log)
            (s: syntax TVar TFn) :=
     match s with
     | Bind var expr body =>
-      opt_bind (interp Gamma rule_log expr) (fun '(rule_log', v) =>
-      interp (putenv Gamma var v) rule_log body)
+      result_bind (interp Sigma Gamma V sched_log rule_log expr) (fun '(rule_log', v) =>
+      interp Sigma (putenv Gamma var v) V sched_log rule_log body)
     | Var var =>
-      opt_map (getenv Gamma var) (fun val => (rule_log, val))
+      result_map (opt_result Stuck (getenv Gamma var)) (fun val => (rule_log, val))
     | Skip =>
-      Some (rule_log, vtt)
+      Success (rule_log, vtt)
     | Const bs =>
-      Some (rule_log, vbits bs)
+      Success (rule_log, vbits bs)
     | If cond tbranch fbranch =>
-      opt_bind (interp Gamma rule_log cond) (fun '(rule_log', condv) =>
+      result_bind (interp Sigma Gamma V sched_log rule_log cond) (fun '(rule_log', condv) =>
       if condv
-      then interp Gamma rule_log' tbranch
-      else interp Gamma rule_log' fbranch)
+      then interp Sigma Gamma V sched_log rule_log' tbranch
+      else interp Sigma Gamma V sched_log rule_log' fbranch)
     | Fail =>
-      None
+      CannotRun
     | Read P0 idx =>
-      let invalid :=
-          orb
-            (List.existsb
-               (fun entry =>
-                  match entry with
-                  | LogRead P1 _ _ | LogWrite _ _ _ _ => true
-                  | _ => false
-                  end) sched_log)
-            (List.existsb
-               (fun entry =>
-                  match entry with
-                  | LogRead P1 _ _ | LogWrite P1 _ _ _ => true
-                  | _ => false
-               end) rule_log) in magic tt
+      result_bind (may_read0 sched_log rule_log idx) (fun _ =>
+      result_map (opt_result Stuck (nth_error V idx)) (fun v =>
+      ((LE LogRead P0 idx vtt) :: rule_log, v)))
     | Read P1 idx =>
-      magic tt
-    | Write P0 idx value =>
-      magic tt
-    | Write P1 idx value =>
-      magic tt
+      result_bind (may_read1 sched_log rule_log idx) (fun latest_w0 =>
+      result_map (opt_result Stuck (nth_error V idx)) (fun v =>
+      ((LE LogRead P1 idx vtt) :: rule_log, match latest_w0 with
+                                           | Some v => v
+                                           | None => v
+                                           end)))
+    | Write lvl idx val =>
+      result_bind (interp Sigma Gamma V sched_log rule_log val) (fun '(rule_log, v) =>
+      result_map (may_write sched_log rule_log lvl idx) (fun _ =>
+      ((LE LogWrite lvl idx v) :: rule_log, vtt)))
     | Call fn args =>
-      opt_bind
+      result_bind
         (List.fold_left
-           (fun (acc: option (Log * list value)) arg =>
-              opt_bind acc (fun '(rule_log, argvs) =>
-              opt_map (interp Gamma rule_log arg) (fun '(rule_log, argv) =>
+           (fun (acc: result (Log * list value)) arg =>
+              result_bind acc (fun '(rule_log, argvs) =>
+              result_map (interp Sigma Gamma V sched_log rule_log arg) (fun '(rule_log, argv) =>
               (rule_log, argv :: argvs))))
-           args (Some (rule_log, [])))
+           args (Success (rule_log, [])))
         (fun '(rule_log, argvs) =>
-           opt_bind (getenv Sigma fn) (fun fn =>
-           opt_bind (fn argvs) (fun resv =>
-           Some (rule_log, resv))))
+           result_bind (opt_result Stuck (getenv Sigma fn)) (fun fn =>
+           result_bind (opt_result Stuck (fn argvs)) (fun resv =>
+           Success (rule_log, resv))))
     end.
+End Interp.
